Rename [reflects] to [isBool], plus minor changes.

src/bool.v
@@ -9,120 +9,134 @@ Set Universe Polymorphism.
    the other is [is_true], a function of type [bool → Prop].
    On a related topic, stdpp offers [decide : {P} + {¬P}]. *)
 
-Class reflects (b : bool) (P Q : Prop) : Prop :=
-  build_reflects :
-  if b then P else Q.
-Global Hint Mode reflects ! - - : typeclass_instances.
+(* We define [isBool b P Q] to mean that [b = true] implies [P]
+   and [b = false] implies [Q]. We do not require that [Q] be [¬P];
+   this is more flexible and lets us avoid a negation in the lemma
+   [reflect_negb], which could lead to the introduction of double
+   negations. *)
+
+Class isBool (b : bool) (P Q : Prop) : Prop :=
+  build_isBool : if b then P else Q.
+
+Global Hint Mode isBool ! - - : typeclass_instances.
   (* Instantiate the parameter [b] only if its head is already known,
      that is, not a metavariable. The other two parameters are outputs. *)
 
-(* TODO rename *)
-Global Notation reflects1 b P :=
-  (reflects b P (¬P)).
+(* In the fairly common case where [Q] is [¬P], we write [isBool1 P]. *)
 
-Global Instance reflects_andb b1 P1 Q1 b2 P2 Q2 :
-  reflects b1 P1 Q1 →
-  reflects b2 P2 Q2 →
-  reflects (andb b1 b2) (P1 ∧ P2) (Q1 ∨ Q2).
-Proof.
-  unfold reflects. destruct b1, b2; simpl; tauto.
-Qed.
+Global Notation isBool1 b P :=
+  (isBool b P (¬P)).
 
-Global Instance reflects_orb b1 P1 Q1 b2 P2 Q2 :
-  reflects b1 P1 Q1 →
-  reflects b2 P2 Q2 →
-  reflects (orb b1 b2) (P1 ∨ P2) (Q1 ∧ Q2).
-Proof.
-  unfold reflects. destruct b1, b2; simpl; tauto.
-Qed.
+(* The tactic [isBool] attempts to prove a goal of the form
+   [isBool b ?P ?Q] using type class search. *)
 
-Global Instance reflects_negb b P Q :
-  reflects b P Q →
-  reflects (negb b) Q P.
-Proof.
-  unfold reflects. destruct b; simpl; tauto.
-Qed.
-
-Lemma reflects_intro b P :
-  (b = true) ↔ P →
-  reflects b P (¬P).
-Proof.
-  assert (false ≠ true) by congruence.
-  unfold reflects. destruct b; simpl; tauto.
-Qed.
-
-Global Instance reflects_intro_true P Q :
-  P →
-  reflects true P Q.
-Proof.
-  unfold reflects. tauto.
-Qed.
-
-Global Instance reflects_intro_false P Q :
-  Q →
-  reflects false P Q.
-Proof.
-  unfold reflects. tauto.
-Qed.
-
-(* TODO remove? *)
-Lemma reflects_elim_true b P Q :
-  b = true →
-  reflects b P Q →
-  P.
-Proof.
-  unfold reflects. intros. subst. tauto.
-Qed.
-
-Lemma reflects_elim_false b P Q :
-  b = false →
-  reflects b P Q →
-  Q.
-Proof.
-  unfold reflects. intros. subst. tauto.
-Qed.
-
-Lemma reflects_conseq b P P' Q Q' :
-  reflects b P Q →
-  (P ↔ P') →
-  (Q ↔ Q') →
-  reflects b P' Q'.
-Proof.
-  unfold reflects. destruct b; tauto.
-Qed.
-
-Lemma reflects1_conseq b P P' :
-  reflects1 b P →
-  (P ↔ P') →
-  reflects1 b P'.
-Proof.
-  unfold reflects. destruct b; tauto.
-Qed.
-
-(* The tactic [reflects] attempts to prove a goal of the form
-   [reflects b ?P ?Q] using type class search. *)
-
-Ltac reflects :=
+Global Ltac isBool :=
   eauto with typeclass_instances.
 
-(* The tactic [reflects_magic] looks for a hypothesis of the form [?b = true]
-   or [?b = false] and transforms it into a hypothesis of the form [P] or [Q]
-   provided type class search finds a fact of the form [reflects b P Q]. *)
+(* The next three lemmas construct [P] and [Q] by examination of [b]. *)
 
-Ltac reflects_magic :=
+Global Instance isBool_andb b1 P1 Q1 b2 P2 Q2 :
+  isBool b1 P1 Q1 →
+  isBool b2 P2 Q2 →
+  isBool (andb b1 b2) (P1 ∧ P2) (Q1 ∨ Q2).
+Proof.
+  unfold isBool. destruct b1, b2; simpl; tauto.
+Qed.
+
+Global Instance isBool_orb b1 P1 Q1 b2 P2 Q2 :
+  isBool b1 P1 Q1 →
+  isBool b2 P2 Q2 →
+  isBool (orb b1 b2) (P1 ∨ P2) (Q1 ∧ Q2).
+Proof.
+  unfold isBool. destruct b1, b2; simpl; tauto.
+Qed.
+
+Global Instance isBool_negb b P Q :
+  isBool b P Q →
+  isBool (negb b) Q P.
+Proof.
+  unfold isBool. destruct b; simpl; tauto.
+Qed.
+
+(* The next three lemmas are currently unused. *)
+
+Lemma isBool_intro b P :
+  (b = true) ↔ P →
+  isBool b P (¬P).
+Proof.
+  assert (false ≠ true) by congruence.
+  unfold isBool. destruct b; simpl; tauto.
+Qed.
+
+Lemma isBool_intro_true P Q :
+  P →
+  isBool true P Q.
+Proof.
+  unfold isBool. tauto.
+Qed.
+
+Lemma isBool_intro_false P Q :
+  Q →
+  isBool false P Q.
+Proof.
+  unfold isBool. tauto.
+Qed.
+
+(* These two lemmas are currently unused. *)
+
+Lemma isBool_conseq b P P' Q Q' :
+  isBool b P Q →
+  (P ↔ P') →
+  (Q ↔ Q') →
+  isBool b P' Q'.
+Proof.
+  unfold isBool. destruct b; tauto.
+Qed.
+
+Lemma isBool1_conseq b P P' :
+  isBool1 b P →
+  (P ↔ P') →
+  isBool1 b P'.
+Proof.
+  unfold isBool. destruct b; tauto.
+Qed.
+
+(* The next two lemmas are used in the tactic [isBool_magic]. *)
+
+Lemma isBool_elim_true b P Q :
+  b = true →
+  isBool b P Q →
+  P.
+Proof.
+  unfold isBool. intros. subst. tauto.
+Qed.
+
+Lemma isBool_elim_false b P Q :
+  b = false →
+  isBool b P Q →
+  Q.
+Proof.
+  unfold isBool. intros. subst. tauto.
+Qed.
+
+(* The tactic [isBool_magic] looks for a hypothesis of the form [?b = true]
+   or [?b = false] and transforms it into a hypothesis of the form [P] or [Q]
+   provided type class search finds a fact of the form [isBool b P Q]. *)
+
+Global Ltac isBool_magic :=
   match goal with
   | h: ?b = true |- _ =>
       let P := fresh in
       evar (P : Prop);
       assert (P); [
-        eapply (@reflects_elim_true b); [ exact h | reflects ]
+        eapply (@isBool_elim_true b); [ exact h | isBool ]
       | clear h; subst P
       ]
   | h: ?b = false |- _ =>
       let P := fresh in
       evar (P : Prop);
       assert (P); [
-        eapply (@reflects_elim_false b); [ exact h | reflects ]
+        eapply (@isBool_elim_false b); [ exact h | isBool ]
       | clear h; subst P
       ]
   end.
